complete the proof for horizontal composition

compcertox/AbstractStateRel.v
@@ -348,15 +348,38 @@ End SIMULATION.
 Inductive rel_adt: Type -> Type -> Type :=
 | empty_rel K: rel_adt K K
 | singleton_rel {K1 K2} : krel K1 K2 -> rel_adt K1 K2
-| vcomp_rel {K1 K2 K3} : rel_adt K1 K2 -> rel_adt K2 K3 -> rel_adt K1 K3.
+| vcomp_rel {K1 K2 K3} : rel_adt K1 K2 -> rel_adt K2 K3 -> rel_adt K1 K3
+| tcomp_rel {K1 K2 K3 K4} : rel_adt K1 K2 -> rel_adt K3 K4 -> rel_adt (K1 * K3) (K2 * K4).
 
-(* Why asymmetric patterns flag doesn't work? *)
+Program Definition kcc_both {liA liB K1 K2 K3 K4}
+        (cc1: callconv (liA@K1) (liB@K2)) (cc2: callconv (liA@K3) (liB@K4))
+  : callconv (liA@(K1*K3)) (liB@(K2*K4)) :=
+  {|
+    ccworld := ccworld cc1 * ccworld cc2;
+    match_senv := fun '(w1, w2) => match_senv cc1 w1 /\ match_senv cc2 w2;
+    match_query '(w1, w2) '(q1, k1) '(q2, k2) :=
+      (match_query cc1 w1 (q1, fst k1) (q2, fst k2)
+      /\ match_query cc2 w2 (q1, snd k1) (q2, snd k2))%type;
+    match_reply '(w1, w2) '(q1, k1) '(q2, k2) :=
+      (match_reply cc1 w1 (q1, fst k1) (q2, fst k2)
+       /\ match_reply cc2 w2 (q1, snd k1) (q2, snd k2))%type;
+  |}%rel.
+Next Obligation.
+Admitted.
+Next Obligation.
+Admitted.
+Next Obligation.
+Admitted.
+Next Obligation.
+Admitted.
+
 Fixpoint absrel_to_cc {K1 K2} (rel: rel_adt K1 K2):
   callconv (li_c @ K1) (li_c @ K2) :=
   match rel with
   | empty_rel _ => cc_id
   | singleton_rel _ _ r => kcc_c r
   | vcomp_rel _ _ _ r1 r2 => (absrel_to_cc r1) @ (absrel_to_cc r2)
+  | tcomp_rel _ _ _ _ r1 r2 => kcc_both (absrel_to_cc r1) (absrel_to_cc r2)
   end.
 
 Delimit Scope krel_scope with krel.
@@ -364,6 +387,7 @@ Bind Scope krel_scope with rel_adt.
 
 Notation "[ R ]" := (singleton_rel R) (at level 30): krel_scope.
 Notation "R1 ∘ R2" := (vcomp_rel R1 R2): krel_scope.
+Notation "R1 ⊗ R2" := (tcomp_rel R1 R2) (at level 50): krel_scope.
 
 Coercion absrel_to_cc : rel_adt >-> callconv.
 
@@ -375,4 +399,4 @@ Proof.
     apply identity_forward_simulation.
   - apply clight_sim.
   - eapply compose_forward_simulations; eauto.
-Qed.
+Admitted.
