compcertox/CModule.v
@@ -132,55 +132,42 @@ Section APP.
         * cbn in *. apply IHps.
   Qed.
 
-  Context `{!CategoricalLinkable (semantics M sk) (semantics N sk)}.
+  Section CAT_APP.
+    Context `{!CategoricalLinkable (semantics M sk) (semantics N sk)}.
 
-  Lemma cmodule_app_simulation:
-    comp_semantics' (semantics M sk) (semantics N sk) sk ≤ semantics (M ++ N) sk.
-  Proof.
-    etransitivity.
-    apply categorical_compose_approximation; typeclasses eauto.
-    fold L. rewrite Leq.
-    etransitivity. apply level_simulation1.
-    etransitivity. eapply bijective_map_simulation1 with (F := F).
-    apply FG_bij. unfold semantics. rewrite <- LFeq.
-    (* FIXME: add typeclass *)
-    apply identity_forward_simulation.
-  Qed.
+    Lemma cmodule_app_simulation:
+      comp_semantics' (semantics M sk) (semantics N sk) sk ≤ semantics (M ++ N) sk.
+    Proof.
+      etransitivity.
+      apply categorical_compose_approximation; typeclasses eauto.
+      fold L. rewrite Leq.
+      etransitivity. apply level_simulation1.
+      etransitivity. eapply bijective_map_simulation1 with (F := F).
+      apply FG_bij. unfold semantics. rewrite <- LFeq.
+      reflexivity.
+    Qed.
+  End CAT_APP.
+
+  Section FLAT_APP.
+    Context `{!FlatLinkable L}.
+
+    Lemma cmodule_flat_comp_simulation:
+      flat_comp_semantics' L sk ≤ semantics (M ++ N) sk.
+    Proof.
+      etransitivity.
+      apply flat_composition_approximation;
+        [ intros [|]; typeclasses eauto
+        | eauto | decide equality ].
+      rewrite Leq.
+      fold @SmallstepLinking_.semantics.
+      etransitivity. apply level_simulation1.
+      etransitivity. eapply bijective_map_simulation1 with (F := F).
+      apply FG_bij. unfold semantics. rewrite <- LFeq.
+      reflexivity.
+    Qed.
+  End FLAT_APP.
 
 End APP.
-
-Section LIFT_COMPONENT.
-  Generalizable All Variables.
-  Context `{L1: Smallstep_.semantics liB liC}
-          `{L2: Smallstep_.semantics liA liB}.
-  Variable (sk sk': AST.program unit unit).
-
-  Let L2' := skel_extend L2 sk'.
-  Inductive state_match: comp_state L1 L2' -> comp_state L1 L2 -> Prop :=
-  | match1 s1: state_match (st1 L1 L2' s1) (st1 L1 L2 s1)
-  | match2 s1 s2: state_match (st2 L1 L2' s1 s2) (st2 L1 L2 s1 s2).
-  Hint Constructors state_match.
-
-  Lemma lift_comp_component:
-    comp_semantics' L1 (skel_extend L2 sk') sk ≤ comp_semantics' L1 L2 sk.
-  Proof.
-    constructor. econstructor. reflexivity. intros. reflexivity.
-    intros se ? [ ] [ ] Hse.
-    instantiate (1 := fun _ _ _ => _). cbn beta.
-    eapply forward_simulation_step with (match_states := state_match).
-    - intros. inv H. inv H0. eexists; split; try constructor; eauto.
-    - intros. inv H0. inv H. eexists; split; try constructor; eauto.
-    - intros. inv H0. inv H. eexists tt, _.
-      repeat apply conj; try constructor; eauto.
-      intros. inv H. inv H0. eexists; split; try constructor; eauto.
-    - intros. inv H; inv H0.
-      + eexists; split. apply CategoricalComp.step1; eauto. auto.
-      + eexists; split. apply CategoricalComp.step2; eauto. auto.
-      + eexists; split. eapply CategoricalComp.step_push; eauto. auto.
-      + eexists; split. eapply CategoricalComp.step_pop; eauto. auto.
-    - apply well_founded_ltof.
-  Qed.
-End LIFT_COMPONENT.
 
 Lemma cmodule_app_simulation' M N sk sk':
   CategoricalLinkable (semantics M sk) (semantics N sk) -> linkorder sk' sk ->
@@ -188,9 +175,9 @@ Lemma cmodule_app_simulation' M N sk sk':
 Proof.
   intros Hsk.
   etransitivity. 2:{ apply cmodule_app_simulation; auto. }
-  etransitivity. 2:{ apply lift_comp_component. }
+  etransitivity. 2:{ apply lift_comp_component2. }
   eapply categorical_compose_simulation';
-                   [ apply identity_forward_simulation
+                   [ reflexivity
                    | apply identity_forward_simulation
                    | apply linkorder_refl | auto ].
 Qed.
